dafny/top-down/bijective_map.dfy
@@ -1,17 +1,19 @@
 module BijectiveMap {
-    datatype BijectiveMap<T1, T2> = BijectiveMap(l_to_r:map<T1, T2>, r_to_l:map<T2, T1>) {
+    datatype BijectiveMap<T1(!new), T2(!new)> = BijectiveMap(l_to_r:map<T1, T2>, r_to_l:map<T2, T1>) {
         predicate valid() {
-            (forall k:T1 | k in l_to_r :: 
+            (forall k:T1 :: k in l_to_r ==>
                 l_to_r[k] in r_to_l && r_to_l[l_to_r[k]] == k)
-            && (forall k:T2 | k in r_to_l :: 
+            && (forall k:T2 :: k in r_to_l ==> 
                 r_to_l[k] in l_to_r && l_to_r[r_to_l[k]] == k)
+            // && (forall t1:T1, t2:T2 :: (t1, t2) in l_to_r.Items ==> (t2, t1) in r_to_l.Items)
+            // && (forall t1:T1, t2:T2 :: (t2, t1) in r_to_l.Items ==> (t1, t2) in l_to_r.Items)
         }
 
         lemma same_size()
             requires valid()
             ensures |l_to_r| == |r_to_l|
         {
-            assert(|l_to_r| == |r_to_l|);
+            assert(|l_to_r.Items| == |r_to_l.Items|);
         }
 
         // method foo() 
