dafny/top-down/search_clause.dfy
@@ -7,23 +7,23 @@ import opened Wrappers
 import opened Seq
 import opened BijectiveMap
 
-datatype SearchClause = SearchClause(name:string, evar_terms:seq<Evar>, rule: Rule, bimap:BijectiveMap<VarTerm, Evar>)
+datatype SearchClause = SearchClause(name:string, evar_terms:seq<Evar>, rule: Rule, subst: EvarSubstitution)
 {
-    predicate valid()
-    {
-        rule.head.name == name
-        // Todo something about the body mapping to the rule's body under some evar map
-    }
-    function subst_of() : Substitution
-        ensures rule.head.substitution_concrete(subst_of())
-        ensures (forall clause :: clause in rule.body ==> 
-                        clause.substitution_concrete(subst_of()))
-    {
-        //bimap.l_to_r
-        assume false;
-        map[]
-        // todo something about applying it to an evar_map to get an actual concrete subst out of it
-    }
+    // predicate valid()
+    // {
+    //     rule.head.name == name
+    //     // Todo something about the body mapping to the rule's body under some evar map
+    // }
+    // function subst_of() : Substitution
+    //     ensures rule.head.substitution_concrete(subst_of())
+    //     ensures (forall clause :: clause in rule.body ==> 
+    //                     clause.substitution_concrete(subst_of()))
+    // {
+    //     //bimap.l_to_r
+    //     assume false;
+    //     map[]
+    //     // todo something about applying it to an evar_map to get an actual concrete subst out of it
+    // }
 
   // predicate is_ground() 
   // {
